\section{Theorie}
\label{sec:Theorie}

\begin{equation}
  V = \frac{B}{G} = \frac{b}{g}
  \label{eqn:AG}
\end{equation}

\begin{equation}
  \frac{1}{f} = \frac{1}{b} + \frac{1}{g}
  \label{eqn:LG}
\end{equation}

\begin{equation}
  f = \frac{e^2 - d^2}{4e}
  \label{eqn:bessel}
\end{equation}

\begin{equation}
  g' = g + h = f \cdot \left( 1 + \frac{1}{V}\right) + h
  \qquad
  h' = b + h' = f \cdot \left( 1+ V \;\right) + h'
  \label{eqn:abbe}
\end{equation}

\begin{equation}
   D =  \sum_i ^N D_i
  \label{eqn:D}
\end{equation}
